checkpoint; most of new_invariant

pulse/lib/pulse/core/PulseCore.Heap.fst
@@ -86,6 +86,19 @@ let core_ref_null = Null
 
 let core_ref_is_null (r:core_ref) = Null? r
 
+let addr_as_core_ref n = Addr n
+let core_ref_as_addr (c:core_ref) =
+  match c with
+  | Null -> 0
+  | Addr n -> n
+
+let addr_core_ref_injective (n:nat)
+: Lemma (core_ref_as_addr (addr_as_core_ref n) == n)
+= ()
+let addr_core_ref_injective_2 (c:core_ref { not (core_ref_is_null c) })
+: Lemma (addr_as_core_ref (core_ref_as_addr c) == c)
+= ()
+
 let disjoint (m0 m1:heap u#h)
   : prop
   = forall a. disjoint_addr m0 m1 a
@@ -688,6 +701,10 @@ let heap_evolves : FStar.Preorder.preorder full_heap =
 let free_above_addr h a =
   forall (i:nat). i >= a ==> h i == None
 
+let interp_free_above (h:heap u#a) (a:nat)
+: Lemma (free_above_addr h a <==> (forall i. i >= a ==> select i h == None))
+= ()
+
 let weaken_free_above (h:heap) (a b:nat)
   : Lemma (free_above_addr h a /\ a <= b ==> free_above_addr h b)
   = ()
@@ -1160,6 +1177,18 @@ let extend #a #pcm
         (x:a{pcm.refine x})
         (addr:nat)
  = refined_pre_action_as_action (extend_alt x addr)
+
+let extend_modifies_nothing
+      #a #pcm (x:a { pcm.refine x })
+      (addr:nat) (h:full_hheap emp { free_above_addr h addr })
+: Lemma (
+      let (| r, h1 |) = extend #a #pcm x addr h in
+      (forall (a:nat). a <> addr ==> select a h == select a h1) /\
+      select addr h1 == Some (Ref a pcm Frac.full_perm x) /\
+      not (core_ref_is_null r) /\
+      addr == core_ref_as_addr r
+  )
+= ()
 
 let hprop_sub (p q:slprop) (h0 h1:heap)
   : Lemma (requires (forall (hp:hprop (p `star` q)). hp h0 == hp h1))
